\documentclass[12pt,letterpaper]{article}
\usepackage[utf8]{inputenc}
\usepackage{amsmath}
\usepackage{amsfonts}
\usepackage{amssymb}
\usepackage[cancel}
\author{Shawn Hartley}
\begin{document}
\begin{equation}
F = ma
\end{equation}
\begin{equation}
a = \dfrac{dv}{dt}
\end{equation}
\[\begin{align}


F_{\textbf{gravity towards center of planet}} = -m\cdot g\\

F_{\textbf{resisting gravity}} = m\cdot g\\

F_{\textbf{resisting gravity}} = m\cdot g \propto v^{2}\\

F_{\textbf{resisting gravity}} = m\cdot g = k\cdot v^{2}\\

\sum Forces = F_{\textbf{resisting gravity}} + F_{\textbf{resisting gravity}}\\

\sum Forces = k\cdot v^{2} - m\cdot g\\

m\cdot \dfrac{dv}{dt} = k\cdot v^{2} - m\cdot g\\

\int \dfrac{m}{m\cdot g-k\cdot v^{2}}dv = \int dt\\

\dfrac{-\ln\left(\dfrac{\sqrt{k}\cdot v - \sqrt{m\cdot g}}{\sqrt{k}\cdot v + \sqrt{m\cdot g}}\right)}{2\sqrt{m\cdot g\cdot k}} = t + c\\

-\ln \dfrac{\sqrt{k}\cdot v - \sqrt{m\cdot g}}{\sqrt{k}\cdot v + \sqrt{m\cdot g}} = 2\cdot t\sqrt{m\cdot g\cdot k} + c \\

\textit{e}^{-\ln \dfrac{\sqrt{k}\cdot v - \sqrt{m\cdot g}}{\sqrt{k}\cdot v + \sqrt{m\cdot g}}} = \textit{e}^{2\cdot t\sqrt{m\cdot g\cdot k} + c}\\

\left(\dfrac{\sqrt{k}\cdot v - \sqrt{m\cdot g}}{\sqrt{k}\cdot v + \sqrt{m\cdot g}}\right)^{-1} = \textit{e}^{2\cdot t\sqrt{m\cdot g\cdot k}} \textit{e}^{c}\\

\dfrac{\sqrt{k}\cdot v + \sqrt{m\cdot g}}{\sqrt{k}\cdot v - \sqrt{m\cdot g}} = c\cdot \textit{e}^{2\cdot t\sqrt{m\cdot g\cdot k}}\\

\sqrt{k}\cdot v + \sqrt{m\cdot g} = c\textit{e}^{2\cdot t\sqrt{m\cdot g\cdot k}}(\sqrt{k}\cdot v - \sqrt{m\cdot g})\\

\sqrt{k}\cdot v + \sqrt{m\cdot g} = \sqrt{k}\cdot v\cdot c\cdot \textit{e}^{2\cdot t\sqrt{m\cdot g\cdot k}} - \sqrt{m\cdot g}\cdot c\cdot \textit{e}^{2\cdot t\sqrt{m\cdot g\cdot k}}\\

\sqrt{k}\cdot v - \sqrt{k}\cdot v\cdot c\cdot \textit{e}^{2\cdot t\sqrt{m\cdot g\cdot k}} = -\sqrt{m\cdot g}\cdot c \cdot \textit{e}^{2\cdot t\sqrt{m\cdot g\cdot k}} -\sqrt{m\cdot g}\\

v\cdot(\sqrt{k} - \sqrt{k}\cdot c\cdot \textit{e}^{2\cdot t\sqrt{m\cdot g\cdot k}}) = -\sqrt{m\cdot g}\cdot c \cdot \textit{e}^{2\cdot t\sqrt{m\cdot g\cdot k}} -\sqrt{m\cdot g}\\

v = \dfrac{-\sqrt{m\cdot g}\cdot c \cdot \textit{e}^{2\cdot t\sqrt{m\cdot g\cdot k}} -\sqrt{m\cdot g}}{\sqrt{k} - \sqrt{k}\cdot c\cdot \textit{e}^{2\cdot t\sqrt{m\cdot g\cdot k}}}\\
\end{align}
\]

Since the object was released from rest, the initial velocity at $t = 0$ is $v = 0$. Therefore we can easily solve for c.

\[
\texttt{At $t = 0$ and $v = 0$}\\

0 = \dfrac{-c\cdot \sqrt{m\cdot g}\cdot \textit{e}^{2\cdot t\sqrt{m\cdot g\cdot k}} - \sqrt{m\cdot g}}{\sqrt{k}-\sqrt{k}\cdot c}\\

\rightarrow \hspace{5 mm} \dfrac{-\sqrt{m\cdot g}\cdot(c + 1)}{\sqrt{k}\cdot (1-c)}\\

\rightarrow \hspace{5 mm} c = -1\\

\texttt{So}\\

v = \dfrac{\sqrt{m\cdot g}\cdot \textit{e}^{2\cdot t\sqrt{m\cdot g\cdot k}} -\sqrt{m\cdot g}}{\sqrt{k} + \sqrt{k}\cdot \textit{e}^{2\cdot t\sqrt{m\cdot g\cdot k}}}\\

v = \dfrac{\sqrt{m \cdot g}\cdot (\textit{e}^{2\cdot t\sqrt{m\cdot g\cdot k}} - 1)}{\sqrt{k}\cdot (1 + \textit{e}^{2\cdot t\sqrt{m\cdot g\cdot k}})}

\lim_{t\to\infty} \dfrac{\sqrt{m \cdot g}\cdot (\textit{e}^{2\cdot t\sqrt{m\cdot g\cdot k}} - 1)}{\sqrt{k}\cdot (1 + \textit{e}^{2\cdot t\sqrt{m\cdot g\cdot k}})} = \dfrac{\sqrt{m\cdot g}\cdot \infty}{\sqrt{k}\cdot \infty}\\
\]

$\therefore \hspace{5 mm}$ As $t\to\infty$ \hspace{5 mm} $v\to \dfrac{\sqrt{mg}}{\sqrt{k}}$.
\end{document}